new `Experimental` folder

LeanBoogie/Experimental/DijkstraMonadSt.lean
@@ -1,5 +1,14 @@
 import Std
 import Aesop
+import Auto
+import Duper
+
+set_option trace.auto.smt.printCommands true
+set_option trace.auto.smt.result true
+set_option trace.auto.printLemmas true
+set_option auto.smt.trust true
+set_option auto.smt.solver.name "z3"
+set_option pp.fieldNotation.generalized false
 
 -- # Dijkstra Monad for non-ITree StateT
 
@@ -29,24 +38,61 @@ instance : Monad StW := { pure := StW.pure, bind := StW.bind }
 theorem StW.bind_push_state {a : StW A} {b : A -> StW B} {post : B × S -> Prop} {σ : S} : (a >>= b) post σ = a (fun res => b res.fst post res.snd) σ := rfl
 def StW.read : StW Int := fun (post : Int × S → Prop) (s:S) => post (s, s)
 def StW.write (a : Int) : StW Unit := fun (post : Unit × S → Prop) (_:S) => post ((), a)
+def StW.and (v w : StW A) : StW A := fun post s => (v post s) ∧ (w post s)
 
 example : StW.pure 123                             = (fun post s => post (123, s)) := rfl
 example : StW.pure 123 (fun (_, s) => s < 200)     = (fun s => s < 200)            := rfl
 example : StW.pure 123 (fun (n, _) => n = 123) 200                                 := rfl
 
+/-- Allows us to create a specification from arbitrary pre-conditions and post-conditions.
+  Source: [DM4Ever] page 15. -/
+def encode (pre : S -> Prop) (post : (A × S) -> Prop) : StW A :=
+  fun p s => pre s ∧ (∀r, post r -> p r)
+
 -- ## Monad Morphism from M to W / Effect observation
 
-def θ (m : St A) : StW A := fun (post : A × S -> Prop) (s₀ : S) => post (m s₀)
+def θ (m : St A) : StW A :=
+  fun (post : A × S -> Prop) (s₀ : S) =>
+    post (m s₀)
+
 def StW.le (w1 w2 : StW A) : Prop := ∀p s, w2 p s -> w1 p s -- [DM4All 3.1]
 instance : LE (StW A) := ⟨StW.le⟩
--- Important for θ to be a monad morphism [DM4All 3.1]
-theorem θ_bind {a : St A} {b : A -> St B} : θ (a >>= b) = (θ a >>= fun a => θ (b a)) := rfl
 
+-- Important for θ to be a monad morphism [DM4All 3.1]
+theorem θ_pure : θ (return a) = return a := rfl
+theorem θ_bind : θ (a >>= b) = (θ a >>= fun a => θ (b a)) := rfl
+
+def θ_if [Decidable φ] {t e : St A}
+  : θ (if φ then t else e)
+  = if φ then θ t else θ e
+  := by
+  split
+  next h => simp_all only
+  next h => simp_all only
+
+def θ_if' [Decidable φ] {t e : St A}
+  : θ (if φ then t else e)
+  = (fun post s => (φ -> θ t post s) ∧ (¬φ -> θ e post s))
+  := by
+  split
+  next h => simp_all only [true_implies, not_true_eq_false, false_implies, and_true]
+  next h => simp_all only [false_implies, not_false_eq_true, true_implies, true_and]
+
+def θ_read : θ (St.read) = StW.read := rfl
+def θ_write : θ (St.write val) = StW.write val := rfl
+
+theorem verify_ite [Decidable φ] {w t e : StW A}
+  (tru :  φ -> t <= w)
+  (fal : ¬φ -> e <= w)
+  : (if φ then t else e) <= w
+  := by aesop
 
 -- ## (Verification Helper)
 -- Basically the Dijkstra monad, but instead of `.. -> @Subtype M W`, it is `.. -> W -> M -> Prop`
 
 def StV {A : Type} (w : StW A) (m : St A) : Prop := θ m <= w
+instance : Membership (St A) (StW A) := ⟨StV⟩
+def Equivalent (m₁ m₂ : St A) := θ m₁ <= θ m₂  ∧  θ m₂ <= θ m₁
 
 /-- There exists exactly one program which returns `a`. -/
 theorem StV.pure  (a : A) : StV (StW.pure a) (St.pure a) := by
@@ -81,8 +127,11 @@ theorem StV.weaken (weaker : w₁ <= w₂) (mv : StV w₁ m) : StV w₂ m := by
   intro post s h
   simp_all only
 
-def Equivalent (m₁ m₂ : St A) := θ m₁ <= θ m₂  ∧  θ m₂ <= θ m₂
+theorem if_fun_push [Decidable φ] {α β : X -> Y}
+  : (if φ then fun x => α x else fun x => β x) x
+  = (if φ then α x else β x) := by aesop
 
+theorem if_Prop [Decidable φ] : (if φ then α else β) = ((φ -> α) ∧ (¬φ -> β)) := by aesop
 
 /-- ## Dijkstra Monad
   Intuitively: The set of all computations which live up to the specification.
@@ -92,12 +141,12 @@ def Equivalent (m₁ m₂ : St A) := θ m₁ <= θ m₂  ∧  θ m₂ <= θ m₂
   But that is not what we want for equivalanence checking: When equivalence checking, we already
   have a program `m : St A`, and we want to show that it lives up to a spec.
 -/
-def StD (A : Type) (w : StW A) : Type := {m : St A // θ m <= w} -- `θ m <= w` = `StV w m`
+def StD (A : Type) (w : StW A) : Type := {m : St A // θ m <= w}
 def StD.pure (a : A) : StD A (StW.pure a) := ⟨St.pure a, StV.pure a⟩
 def StD.bind {wa : StW A} {wb : A -> StW B} (da : StD A wa) (db : (a:A) -> StD B (wb a)) : StD B (StW.bind wa wb) := ⟨ St.bind da.1 (fun a => (db a).1), StV.bind da.2 (fun a => (db a).2)⟩
-def StD.weaken {w1 w2 : StW A} (weaker : w1 <= w2) : StD A w1 -> StD A w2 := sorry
+def StD.weaken {w1 w2 : StW A} (weaker : w1 <= w2) : StD A w1 -> StD A w2 := fun ⟨m, w⟩ => ⟨m, StV.weaken weaker w⟩
 
-section Example
+namespace Example1
   def p1 : St Unit := do
     let x <- St.read
     St.write (x+2)
@@ -118,6 +167,13 @@ section Example
     simp only [St.read.eq_unfold, St.write.eq_unfold, St.bind_push_state]
     exact h
 
+  example : StV (encode (. = 0) (. = ((), 2))) p1 := by
+    simp [StV, θ.eq_unfold, LE.le, StW.le, encode]
+    intro post h
+    rw [p1]
+    simp only [St.read.eq_unfold, St.write.eq_unfold, St.bind_push_state]
+    exact h
+
   /-- Let's show that p1 increments the state by less than 10.
     Note that `StV w : St _ -> Prop` is a predicate which describes the set of valid computations. -/
   example : StV (fun post s => ∀s' < s + 10, post ((), s')) p1 := by
@@ -127,4 +183,71 @@ section Example
     simp only [St.read.eq_unfold, St.write.eq_unfold, St.bind_push_state]
     have := h_post (s+2) (by unfold S; omega)
     exact this
-end Example
+
+  /-- `θ p1 (fun ((), s') => s' < s + 10) : BoogieState -> Prop` describes the set of initial states
+    for which, after executing p1, the postcondition holds. -/
+  example (s) : θ p1 (fun ((), s') => s' < s + 10) s := by
+    rw [p1]
+    rw [θ_bind]
+    rw [θ.eq_unfold]
+    simp only
+    rw [St.read.eq_unfold, St.write.eq_unfold]
+    simp only [bind, StW.bind]
+    unfold S; omega
+end Example1
+
+namespace Example2
+  def abs : St Int := do
+    if (<- St.read) < 0
+      then return - (<- St.read)
+      else return (<- St.read)
+
+  def abs' : St Int := do
+    let x <- St.read
+    if x >= 0 then return x else return -x
+
+  example : θ abs <= θ abs' := by
+    intro rhs_post s rhs_post_h
+    simp [abs, abs'] at *
+    simp [θ_pure, θ_bind, θ_read, θ_write, θ_if] at *
+    simp [StW.read.eq_unfold, StW.pure.eq_unfold, Pure.pure, Bind.bind, StW.bind.eq_unfold, StW.pure.eq_unfold] at *
+    simp [if_fun_push] at *
+    rw [if_Prop] at *
+    -- rhs_post_h : (0 ≤ s → rhs_post (s, s)) ∧ (¬0 ≤ s → rhs_post (-s, s))
+    -- ⊢ (s < 0 → rhs_post (-s, s)) ∧ (¬s < 0 → rhs_post (s, s))
+    obtain ⟨left, right⟩ := rhs_post_h
+    constructor
+    . sorry
+    . sorry
+end Example2
+
+namespace Example3
+  def f (x : Int) : St Unit := do
+    let a <- St.read
+    St.write (a + x)
+    let a <- St.read
+    St.write (a + x)
+
+  def g (x : Int) : St Unit := do
+    let a <- St.read
+    St.write (a + (2 * x))
+
+  theorem bad_approach : θ (f x) <= θ (g x) := by
+    intro rhs_post s rhs_post_h
+    rw [θ] at * -- bad: we don't want to unfold θ so soon! Only at the leaves.
+    -- Now we have `rhs_post (g x s) ⊢ rhs_post (f x s)` which defeats the purpose of `θ`.
+    simp [f, g] at *
+    -- Now we have `rhs_post_h : rhs_post ((St.read >>= fun tmp => St.write (tmp + 2 * x)) s)`,
+    -- which is not as handy as the better approach
+    sorry
+
+  /- Taking a step back, recall that `θ` is a monad morphism, so it is compatible with `pure`, `bind`.
+    We can thus push θ inwards. -/
+  theorem good_approach : θ (f x) <= θ (g x) := by
+    simp [f, g] at *
+    simp [θ_pure, θ_bind, θ_read, θ_write, θ_if] at *
+    simp [StW.write.eq_unfold, StW.read.eq_unfold, StW.pure.eq_unfold, Pure.pure, Bind.bind, StW.bind.eq_unfold, StW.pure.eq_unfold] at *
+    intro rhs_post s rhs_post_h
+    have : x + x = 2 * x := by omega
+    simp only [this, Int.add_assoc, rhs_post_h]
+end Example3
