LeanBoogie/Experimental/AmAt.lean
@@ -1,0 +1,86 @@
+import LeanBoogie.ITree
+import LeanBoogie.ITree.ITree0W
+
+open ITree
+
+/-- `Assume` effect. You can write programs such as the following, where you obtain a proof of
+  the proposition you're assuming.
+  ```
+  .vis (.read "i") fun (i : Int) =>
+    .vis (.assume (i < 123)) fun (prf : i < 2) =>
+      ...
+  ```
+  It is up to whoever interprets the event stream to provide the actual proof though!
+  For example, if you're executing a memoryful program, you may try to decide the proposition using
+  either a decision procedure or SMT solvers.  But if you can't provide a proof, you get stuck
+  during execution. If you decide the assumption to be false, you are in an impossible branch,
+  so you can safely eliminate that branch, and need not follow it further.
+
+  You can interpret this into a nondeterminism (i.e. set of possible continuations) monad as follows.
+  Namely, the set of all continuations for which we are able to provide a proof.
+  Note that `Pow A = A -> Prop`.
+  ```
+  def interp : ITree (Am + E) A -> Pow (ITree E A)
+  | .vis (.assume P) k => { t : ITree E A | (prf : P) × t = k prf }
+  | ...
+  ```
+
+  If you instead try to observe this into a Dijkstra monad, you kind of fail at first
+  ```
+  def θ : ITree Am A -> ITree0W A :=
+    fun (post : ITree0 A -> Prop) =>
+      (prf : P???) × post ???
+  ```
+
+  *Key insight*: Both the dijkstra monad and the powerset non-deterministic interpretation describe
+    a set of possible computations. Is it the same notion? Only difference is that dijkstra monad
+    also is a predicate transformer.
+
+  So you actually want something like the following. However, if we have effects other than `Am`,
+  it is unknown whether we can write down `ITreeW`. One solution is to interpret e.g. memory effects
+  away before interpreting away `Am`.
+  ```
+  def interp_or_θ : ITree (Am + E) A -> ITree0W A :=
+  | .vis (.assume P) k =>
+    fun (post : ITree Empty A -> Prop) =>
+      (prf : P) -> post (interp_or_θ (k prf))
+  | ...
+  ```
+
+  Now let's denote `if` as a nondet jump to two itrees, each starting with an assumes event:
+  ```
+  def myprog : ITree (Am + Choose + Mem) A :=
+    .vis (.choose (Fin 2)) fun
+      | 0 => .vis (.assume   φ ) fun (prf :  φ) => t
+      | 1 => .vis (.assume (¬φ)) fun (prf : ¬φ) => e
+  ```
+  Then you get something like a `ITreeW Mem A` or an `ITree0W A`, but no more `Choose` and `Am`:
+  ```
+  interp_or_θ myprog = (fun s post => ??)
+  ```
+-/
+inductive Am : Type
+| assume : (P : Prop) -> Am
+
+/-- `Assert` effect. You can write programs such as:
+  ```
+  .vis (.read "i") fun (i : Int) =>
+    .vis (.assert (i < 123)) fun () =>
+      ...
+  ```
+
+  If you interpret this into a nondeterminism monad...
+  ```
+  def interp : ITree (At + E) A -> Pow (ITree E A)
+  | .vis (.assert P) k => { t : ITree E A | t = k ()  ∧  ??? }
+  | ...
+  ```
+-/
+inductive At : Type
+| assert : (P : Prop) -> At
+
+inductive AmAt : Type
+| assume : (P : Prop) -> AmAt
+| assert : (P : Prop) -> AmAt
+
+-- def interp : ITree AmAt A -> ITree0W A
