LeanBoogie/Experimental/State.lean
@@ -1,0 +1,54 @@
+import LeanBoogie.ITree.ITree
+
+/-
+  # State in Boogie
+-/
+
+-- ## Codes for boogie state types
+
+inductive Ty : Type
+| bool
+| int
+| bv (bits : Nat)
+-- | map (A B : Ty)
+
+abbrev Con : Type := List Ty
+-- inductive Con : Type where
+-- | empty : Con
+-- | ext : Con -> Ty -> Con
+
+-- def Var (Γ : Con) : Type := Fin Γ.length
+inductive Var : (Γ : Con) -> (A : Ty) -> Type
+| vz :            Var (A :: Γ) A
+| vs : Var Γ A -> Var (B :: Γ) A
+
+-- ## Interpretations of boogie type codes
+
+def TyA : Ty -> Type
+| .int => Int
+| .bool => Bool
+| .bv bits => BitVec bits
+-- | .map A B => TyA A -> TyA B
+
+def ConA : Con -> Type
+| [] => Unit
+| x :: xs => TyA x × ConA xs
+
+instance : CoeSort Ty Type := ⟨TyA⟩
+instance : CoeSort Con Type := ⟨ConA⟩
+
+-- ## Interaction Tree Events for State
+
+namespace Approach1
+  inductive Mem (Γ : Con) : /- Type -> -/ Type where
+  | rd : Var Γ A          -> Mem Γ /- (TyA A) -/
+  | wr : Var Γ A -> TyA A -> Mem Γ /- Unit -/
+  -- def Mem.read  (v : Var Γ A)           : ITree (Mem Γ) A := .vis (.rd v) (fun a:A => .ret a)
+  -- def Mem.write (v : Var Γ A) (val : A) : ITree (Mem Γ) A := .vis (.wr v val) (fun () => .ret ())
+end Approach1
+
+namespace Approach2
+  inductive Mem (Γ : Type) : /- (A:Type) -> -/ Type where
+  | rd (π : Γ -> Ans) : Mem Γ /- A -/
+  | wr (δ : Γ -> Ans -> Γ) : Mem Γ /- Unit -/
+end Approach2
